switch to ocaml native strings

deps/poulet4/examples/IntExample.v
@@ -1,22 +1,23 @@
 Require Import Syntax.
 Require Import Eval.
 Require Import Typed.
-Require Import CamlString.
 Require Import Strings.String.
+Require String.
 Require Import Coq.ZArith.BinIntDef.
 Require Import Monads.State.
 
 Require Import Step.
 
 Open Scope list_scope.
+Open Scope string_scope.
 
 Definition tag_t := unit.
 Definition tag := tt.
 Definition constTyp : P4Type := TypInteger.
-Definition name : P4String tag_t := MkP4String tag_t tag (caml_string_of_chars "hello_world").
+Definition name : P4String tag_t := MkP4String tag_t tag "hello_world".
 Definition value : ValueBase tag_t := ValBaseInteger tag_t 42.
 
-Definition parses (p: ValueObject tag_t) (fuel: nat) (start_state: caml_string) (start_env: Environment.environment tag_t): bool :=
+Definition parses (p: ValueObject tag_t) (fuel: nat) (start_state: String.t) (start_env: Environment.environment tag_t): bool :=
   match run_with_state start_env (step_trans tag_t tag p fuel start_state) with
   | (inl _, _) => true
   | _ => false
@@ -36,65 +37,79 @@ parser IntExample (packet_in pkt, out int output) {
 }
 *)
 
-Definition scope : Env_EvalEnv := MkEnv_EvalEnv nil nil (caml_string_of_chars "dummy").
+Definition scope : Env_EvalEnv := MkEnv_EvalEnv nil nil "dummy".
 (* Definition good_scope : Env_EvalEnv := MkEnv_EvalEnv  *)
 
-Definition pkt_param : P4Parameter := MkParameter true Directionless (TypExtern (caml_string_of_chars "packet_in")) (caml_string_of_chars "pkt").
+Definition pkt_param : P4Parameter := MkParameter true Directionless (TypExtern "packet_in") "pkt".
 Definition out_type : P4Type := TypInt 2.
-Definition out_param : P4Parameter := MkParameter true Out out_type (caml_string_of_chars "output").
+Definition out_param : P4Parameter := MkParameter true Out out_type "output".
 Definition locals : list (Declaration tag_t) := nil.
-Definition accept_st : ParserState tag_t := MkParserState _ tt (MkP4String _ tt StrConstants.accept) nil (ParserDirect _ tt (MkP4String _ tt StrConstants.accept)).
-Definition output_expr : Expression tag_t := MkExpression _ tt (ExpName _ (BareName (caml_string_of_chars "output"))) out_type Directionless.
-Definition pkt_extract_expr : Expression tag_t := MkExpression _ tt (ExpName _ (BareName (caml_string_of_chars "pkt"))) (TypFunction (MkFunctionType nil ((MkParameter false Directionless out_type (caml_string_of_chars "x"))::nil) FunBuiltin out_type)) Directionless.
+Definition accept_st : ParserState tag_t := MkParserState _ tt (MkP4String _ tt String.accept) nil (ParserDirect _ tt (MkP4String _ tt String.accept)).
+Definition output_expr : Expression tag_t := MkExpression _ tt (ExpName _ (BareName "output")) out_type Directionless.
+Definition pkt_extract_expr : Expression tag_t := MkExpression _ tt (ExpName _ (BareName "pkt")) (TypFunction (MkFunctionType nil ((MkParameter false Directionless out_type "x")::nil) FunBuiltin out_type)) Directionless.
 Definition extract_stmt : Statement tag_t := 
-  MkStatement _ tt (StatMethodCall _ (MkExpression _ tt (ExpExpressionMember _ pkt_extract_expr (MkP4String _ tt StrConstants.extract)) TypVoid Directionless) (out_type :: nil) (Some output_expr :: nil)) StmVoid.
+  MkStatement _ tt (StatMethodCall _ (MkExpression _ tt (ExpExpressionMember _ pkt_extract_expr (MkP4String _ tt String.extract)) TypVoid Directionless) (out_type :: nil) (Some output_expr :: nil)) StmVoid.
 
 
 Definition body: list (Statement tag_t) := extract_stmt :: nil.
-Definition start_st : ParserState tag_t := MkParserState _ tt (MkP4String _ tt (caml_string_of_chars "start")) body (ParserDirect _ tt (MkP4String _ tt StrConstants.accept)).
+Definition start_st : ParserState tag_t := MkParserState _ tt (MkP4String _ tt "start") body (ParserDirect _ tt (MkP4String _ tt String.accept)).
 
 Definition states : list (ParserState tag_t) := start_st :: nil.
 
 Definition IntParser : ValueObject tag_t := ValObjParser _ scope nil nil states.
 
-Lemma caml_string_eqb_true : forall s: string, caml_string_eqb (caml_string_of_chars s) (caml_string_of_chars s) = true.
-Admitted.
-Lemma caml_string_eqb_false : forall s1 s2: string, s1 <> s2 -> caml_string_eqb (caml_string_of_chars s1) (caml_string_of_chars s2) = false.
-Admitted.
-
 Definition bad_env : Environment.environment tag_t := nil.
 
-Lemma int_parses_fail : parses IntParser 2 (caml_string_of_chars "start") bad_env = false.
+Lemma int_parses_fail : parses IntParser 2 "start" bad_env = false.
 Proof.
-  repeat (cbv || rewrite caml_string_eqb_true).
-  auto.
+  reflexivity.
 Qed.
 
 Definition pkt_value : Value tag_t := ValObj _ (ValObjPacket _ (true :: true :: nil)).
 Definition out_value : Value tag_t := ValBase _ (ValBaseInteger _ 0).
 Definition top_scope : Environment.scope tag_t := 
-  Environment.extend_scope _ (caml_string_of_chars "pkt") pkt_value (
-    Environment.extend_scope _ (caml_string_of_chars "output") out_value (
+  Environment.extend_scope _ "pkt" pkt_value (
+    Environment.extend_scope _ "output" out_value (
       Environment.MStr.empty _
     )
   ).
 
 Definition inter_scope : Environment.scope tag_t := 
-  Environment.MStr.add (caml_string_of_chars "pkt")
+  Environment.MStr.add "pkt"
                               (ValObj tag_t (ValObjPacket tag_t nil))
                               top_scope.
-Definition good_env : Environment.environment tag_t := top_scope :: nil.
+Definition good_env: Environment.environment tag_t := top_scope :: nil.
 
-Lemma top_find_pkt : Environment.MStr.find (caml_string_of_chars "pkt") top_scope = Some pkt_value.
-Admitted.
-Lemma top_find_val : Environment.MStr.find (caml_string_of_chars "output") top_scope = Some out_value.
-Admitted.
-Lemma top_find_val_inter : Environment.MStr.find (caml_string_of_chars "output") inter_scope = Some out_value.
-Admitted.
-
-
-Lemma int_parses : parses IntParser 2 (caml_string_of_chars "start") good_env = true.
+Lemma top_find_pkt: Environment.MStr.find "pkt" top_scope = Some pkt_value.
 Proof.
+  unfold top_scope, Environment.extend_scope.
+  apply Environment.MStr.find_1.
+  now apply Environment.MStr.add_1.
+Qed.
+Lemma top_find_val : Environment.MStr.find "output" top_scope = Some out_value.
+Proof.
+  unfold top_scope, Environment.extend_scope.
+  apply Environment.MStr.find_1.
+  apply Environment.MStr.add_2;
+    [congruence|].
+  now apply Environment.MStr.add_1.
+Qed.
+
+Lemma top_find_val_inter : Environment.MStr.find "output" inter_scope = Some out_value.
+Proof.
+  unfold top_scope, Environment.extend_scope.
+  apply Environment.MStr.find_1.
+  apply Environment.MStr.add_2; [congruence|].
+  apply Environment.MStr.add_2; [congruence|].
+  now apply Environment.MStr.add_1.
+Qed.
+
+Hint Rewrite top_find_pkt top_find_val top_find_val_inter: int_example.
+
+Lemma int_parses : parses IntParser 2 "start" good_env = true.
+Proof.
+  unfold parses.
+  simpl.
   unfold IntParser.
   unfold states.
   unfold start_st.
@@ -108,7 +123,7 @@ Proof.
 
   unfold step.
   unfold lookup_state.
-  rewrite caml_string_eqb_true.
+  simpl.
   unfold Monad.mbind. unfold state_monad_inst. unfold state_bind.
   unfold body. 
 
@@ -146,9 +161,9 @@ Proof.
 
   unfold Monad.mret. unfold state_monad_inst. unfold state_return.
   unfold pkt_value.
-  unfold StrConstants.extract.
+  unfold String.extract.
 
-  rewrite caml_string_eqb_true.
+  simpl.
   unfold extract_value_func. unfold eval_builtin_func.
 
   unfold Monad.mbind. unfold state_monad_inst. unfold state_bind.
@@ -171,14 +186,14 @@ Proof.
 
   unfold Monad.mret. unfold state_monad_inst. unfold state_return.
 
-  unfold StrConstants.extract. 
-  unfold StrConstants.isValid. rewrite caml_string_eqb_false.
-  unfold StrConstants.setValid. rewrite caml_string_eqb_false.
-  unfold StrConstants.setInvalid. rewrite caml_string_eqb_false.
-  unfold StrConstants.pop_front. rewrite caml_string_eqb_false.
-  unfold StrConstants.push_front. rewrite caml_string_eqb_false.
+  unfold String.extract. 
+  unfold String.isValid.
+  unfold String.setValid.
+  unfold String.setInvalid.
+  unfold String.pop_front. simpl.
+  unfold String.push_front. simpl.
   unfold is_packet_func.
-  unfold StrConstants.extract. rewrite caml_string_eqb_true.
+  unfold String.extract. 
 
   unfold Environment.dummy_value.
   unfold eval_packet_func.
@@ -198,7 +213,7 @@ Proof.
   unfold Monad.mret. unfold state_monad_inst. unfold state_return.
 
   unfold pkt_value.
-  unfold StrConstants.extract. rewrite caml_string_eqb_true.
+  unfold String.extract. simpl in *.
   unfold Packet.eval_packet_extract_fixed.
   unfold out_type.
 
@@ -244,13 +259,8 @@ Proof.
   unfold Environment.pop_scope.
   unfold eval_transition.
   unfold Monad.mret. unfold state_monad_inst. unfold state_return.
-  unfold StrConstants.accept. 
-  rewrite caml_string_eqb_true.
+  unfold String.accept. 
+  simpl.
   auto.
-  rewrite <- String.eqb_neq. auto.
-  rewrite <- String.eqb_neq. auto.
-  rewrite <- String.eqb_neq. auto.
-  rewrite <- String.eqb_neq. auto.
-  rewrite <- String.eqb_neq. auto.
 Qed.
 
