deps/poulet4/extraction/Extract.v
@@ -1,18 +1,8 @@
 Require Import Coq.extraction.ExtrOcamlBasic.
-Require Import Coq.extraction.ExtrOcamlString.
+Require Import Coq.extraction.ExtrOcamlNativeString.
 Require Import Coq.extraction.ExtrOcamlNatInt.
 Require Syntax.
 Require Extraction.
-
-Extract Constant CamlString.caml_string => "string".
-Extract Constant CamlString.caml_string_cmp =>
-  "(fun x y -> let c = String.compare x y in
-               if c < 0 then LT
-               else if c = 0 then EQ
-               else if c > 0 then GT)".
-Extract Constant CamlString.caml_string_eqb => "(=)".
-Extract Constant CamlString.caml_string_of_chars =>
-  "(fun cs -> String.init (List.length cs) (fun n -> List.nth n cs)".
 
 Cd "extraction/lib/".
 Separate Extraction Syntax.
