deps/poulet4/lib/Step.v
@@ -4,7 +4,7 @@ Require Import Eval.
 Require Import Environment.
 Require Import Monads.Monad.
 Require Import Monads.State.
-Require Import CamlString.
+Require String.
 
 Open Scope monad.
 
@@ -15,17 +15,17 @@ Section Step.
   Definition states_to_block (ss: list (Statement tags_t)) : Block tags_t :=
     List.fold_right (BlockCons _) (BlockEmpty _ tags_dummy) ss.
 
-  Fixpoint lookup_state (states: list (ParserState tags_t)) (name: caml_string) : option (ParserState tags_t) := 
+  Fixpoint lookup_state (states: list (ParserState tags_t)) (name: String.t) : option (ParserState tags_t) := 
     match states with
     | List.nil => None
     | s :: states' =>
       let 'MkParserState _ _ (MkP4String _ _ s_name) _ _ := s in
-      if caml_string_eqb name s_name
+      if String.eqb name s_name
       then Some s
       else lookup_state states' name
     end.
 
-  Definition step (p: (ValueObject tags_t)) (start: caml_string) : env_monad tags_t caml_string := 
+  Definition step (p: (ValueObject tags_t)) (start: String.t) : env_monad tags_t String.t := 
     match p with
     | ValObjParser _ env params locals states =>
       match lookup_state states start with
@@ -44,13 +44,13 @@ Section Step.
   always makes forward progress then there exists a fuel value for which
   the parser either rejects or accepts (or errors, but not due to lack of fuel) 
    *)
-  Fixpoint step_trans (p: ValueObject tags_t) (fuel: nat) (start: caml_string) : env_monad tags_t unit := 
+  Fixpoint step_trans (p: ValueObject tags_t) (fuel: nat) (start: String.t) : env_monad tags_t unit := 
     match fuel with 
     | 0   => state_fail Internal (* TODO: add a separate exception for out of fuel? *)
     | S x => let* state' := step p start in 
-            if caml_string_eqb state' StrConstants.accept
+            if String.eqb state' String.accept
             then mret tt
-            else if caml_string_eqb state' StrConstants.reject
+            else if String.eqb state' String.reject
             then state_fail Reject
             else step_trans p x state'
     end.
